Revert "Merge branch 'master' into SP_submission"
This reverts commit 5be588a06229d2b7d9d8d2e008ac07cd7b460405, reversing
changes made to 82508c376e81d1cac944b5210d30e9a1f94ee1fa.

latex/Testing.py
@@ -1,0 +1,4 @@
+def assertEqual(expected, actual, message = ""):
+  if (expected != actual):
+    raise Exception("AssertEqual failed: %s != %s. %s"
+                    % (str(expected), str(actual), message))
