readme.md
@@ -1,6 +1,6 @@
 # INSTALL
 
-The theory files work with Isabelle2017 in 64-bits polyml mode.
+The theory files work with Isabelle2017.
 
 To reduce the startup time it is recommended to build a heap image of
 the theories. Add the following to the ROOTS file of Isabelle
@@ -9,7 +9,6 @@ the theories. Add the following to the ROOTS file of Isabelle
 * (path to repo)/generated
 * (path to repo)/core
 * (path to repo)/properties
-* (path to repo)/instantiation
 
 # Folder structure
 
@@ -19,15 +18,13 @@ the theories. Add the following to the ROOTS file of Isabelle
 commutativity lemmas, simplification rules and proof methods.
 
 "properties" contains the definitions and proofs of security
-properties of CHERI. These properties are defined in terms of an 
-abstraction of CHERI. 
-
-"instantiation" contains a mapping from CHERI instructions to abstract
-actions and a proof that with this mapping, CHERI satisfies the 
-security properties defined before. 
+properties of CHERI.
 
 "scripts" contains the python scripts that are used to generate part
 of the proofs.
+
+"latex" contains the files necessary to export human readable versions
+of the security properties.
 
 # Licence
 
